Add tests for primitive floats
Add utility ldexp and frexp functions to prevent dealing with the shift of
ldshiftexp and frshiftexp everywhere.

Also move primitive integer tests to place all primitive tests in the
same directory.

theories/Floats/FloatAxioms.v
@@ -17,9 +17,9 @@ Definition Prim2EF f :=
   else if is_zero f then E754_zero (get_sign f)
        else if is_infinity f then E754_infinity (get_sign f)
             else
-              let (r, shiftexp) := frshiftexp f in
-              let m := ldshiftexp r ((of_Z prec)+shift) in
-              let e := ([| shiftexp |]%int63 - prec - [| shift |]%int63)%Z in
+              let (r, exp) := frexp f in
+              let m := ldexp r prec in
+              let e := (exp - prec)%Z in
               match [| to_int63 m |]%int63 with
               | Zpos p => E754_finite false p e
               | Zneg p => E754_finite true p e
@@ -35,7 +35,7 @@ Definition EF2Prim ef :=
   | E754_infinity true => neg_infinity
   | E754_finite s m e =>
     let pm := of_int63 (of_Z (Zpos m)) in
-    let f := ldshiftexp pm ((of_Z e)+shift) in
+    let f := ldexp pm e in
     if s then (-f)%float else f
   end.
 
