test-suite/primitive/float/emulated_conv.v
@@ -1,0 +1,20 @@
+Require Import ZArith Float.
+
+Definition two := Eval compute in (one + one)%float.
+Definition half := Eval compute in (one / two)%float.
+Definition huge := Eval compute in ldexp one (1023)%Z.
+Definition tiny := Eval compute in ldexp one (-1023)%Z.
+Definition denorm := Eval compute in ldexp one (-1074)%Z.
+
+Check (eq_refl : EF2Prim (Prim2EF zero) = zero).
+Check (eq_refl : EF2Prim (Prim2EF neg_zero) = neg_zero).
+Check (eq_refl : EF2Prim (Prim2EF one) = one).
+Check (eq_refl : EF2Prim (Prim2EF (-one)) = (-one)%float).
+Check (eq_refl : EF2Prim (Prim2EF infinity) = infinity).
+Check (eq_refl : EF2Prim (Prim2EF neg_infinity) = neg_infinity).
+Check (eq_refl : EF2Prim (Prim2EF huge) = huge).
+Check (eq_refl : EF2Prim (Prim2EF tiny) = tiny).
+Check (eq_refl : EF2Prim (Prim2EF denorm) = denorm).
+Check (eq_refl : EF2Prim (Prim2EF nan) = nan).
+Check (eq_refl : EF2Prim (Prim2EF two) = two).
+Check (eq_refl : EF2Prim (Prim2EF half) = half).
