test-suite/primitive/float/sqrt.v
@@ -1,0 +1,33 @@
+Require Import ZArith Int63 Float.
+
+Open Scope float_scope.
+
+Definition three := Eval compute in of_int63 3%int63.
+Definition nine := Eval compute in of_int63 9%int63.
+
+Check (eq_refl : sqrt nine = three).
+Definition compute1 := Eval compute in sqrt nine.
+Check (eq_refl : three = three).
+
+Definition huge := Eval compute in ldexp one (1023)%Z.
+Definition tiny := Eval compute in ldexp one (-1023)%Z.
+Definition denorm := Eval compute in ldexp one (-1074)%Z.
+
+Goal (Prim2EF (sqrt huge) = EF64sqrt (Prim2EF huge)).
+  now compute.
+Qed.
+
+Goal (Prim2EF (sqrt tiny) = EF64sqrt (Prim2EF tiny)).
+  now compute.
+Qed.
+
+Goal (Prim2EF (sqrt denorm) = EF64sqrt (Prim2EF denorm)).
+  now compute.
+Qed.
+
+Check (eq_refl : sqrt neg_zero = neg_zero).
+Check (eq_refl : sqrt zero = zero).
+Check (eq_refl : sqrt one = one).
+Check (eq_refl : sqrt (-one) = nan).
+Check (eq_refl : sqrt infinity = infinity).
+Check (eq_refl : sqrt neg_infinity = nan).
